theories/typing.v
@@ -13,69 +13,69 @@ Section Typing.
   (* assume a given set of class definitions *)
   Context `{PDC: ProgDefContext}.
 
-  (* Helping the inference with this notation that hides Δ *)
-  Local Notation "Γ ⊢ s <: t" := (@subtype _ Γ Plain s t) (at level 70, s at next level, no associativity).
-  Local Notation "Γ ⊢ s <D: t" := (@subtype _ Γ Aware s t) (at level 70, s at next level, no associativity).
+  (* Helping the inference with this notation that hides pdefs *)
+  Local Notation "Δ ⊢ s <: t" := (@subtype _ Δ Plain s t) (at level 70, s at next level, no associativity).
+  Local Notation "Δ ⊢ s <D: t" := (@subtype _ Δ Aware s t) (at level 70, s at next level, no associativity).
 
-  (* At class + substitution is `ok` w.r.t. to a set of constraints `Γ` if
+  (* At class + substitution is `ok` w.r.t. to a set of constraints `Δ` if
    * - all the types in the substitution are ok
    * - all the constraints of that class are satisfied.
    *)
-  Inductive ok_ty (Γ: list constraint) : lang_ty → Prop :=
-    | OkInt: ok_ty Γ IntT
-    | OkBool: ok_ty Γ BoolT
-    | OkNothing: ok_ty Γ NothingT
-    | OkMixed: ok_ty Γ MixedT
+  Inductive ok_ty (Δ: list constraint) : lang_ty → Prop :=
+    | OkInt: ok_ty Δ IntT
+    | OkBool: ok_ty Δ BoolT
+    | OkNothing: ok_ty Δ NothingT
+    | OkMixed: ok_ty Δ MixedT
     | OkClass t σ def:
-        (∀ i ty, σ !! i = Some ty → ok_ty Γ ty) →
-        Δ !! t = Some def →
-        (∀ i c, def.(constraints) !! i = Some c → Γ ⊢ (subst_ty σ c.1) <D: (subst_ty σ c.2)) →
-        ok_ty Γ (ClassT t σ)
-    | OkNull: ok_ty Γ NullT
-    | OkNonNull: ok_ty Γ NonNullT
-    | OkUnion s t: ok_ty Γ s → ok_ty Γ t → ok_ty Γ (UnionT s t)
-    | OkInter s t: ok_ty Γ s → ok_ty Γ t → ok_ty Γ (InterT s t)
-    | OkGen n: ok_ty Γ (GenT n)
-    | OkEx t: ok_ty Γ (ExT t)
-    | OkDynamic : ok_ty Γ DynamicT
-    | OkSupportDyn : ok_ty Γ SupportDynT
+        (∀ i ty, σ !! i = Some ty → ok_ty Δ ty) →
+        pdefs !! t = Some def →
+        (∀ i c, def.(constraints) !! i = Some c → Δ ⊢ (subst_ty σ c.1) <D: (subst_ty σ c.2)) →
+        ok_ty Δ (ClassT t σ)
+    | OkNull: ok_ty Δ NullT
+    | OkNonNull: ok_ty Δ NonNullT
+    | OkUnion s t: ok_ty Δ s → ok_ty Δ t → ok_ty Δ (UnionT s t)
+    | OkInter s t: ok_ty Δ s → ok_ty Δ t → ok_ty Δ (InterT s t)
+    | OkGen n: ok_ty Δ (GenT n)
+    | OkEx t: ok_ty Δ (ExT t)
+    | OkDynamic : ok_ty Δ DynamicT
+    | OkSupportDyn : ok_ty Δ SupportDynT
   .
 
   Lemma ok_ty_constraint_elim_ G T:
     ok_ty G T →
-    ∀ Γ Γ', G = Γ ++ Γ' →
-    (∀ i c, Γ' !! i = Some c → Γ ⊢ c.1 <D: c.2) →
-    ok_ty Γ T.
+    ∀ Δ Δ', G = Δ ++ Δ' →
+    (∀ i c, Δ' !! i = Some c → Δ ⊢ c.1 <D: c.2) →
+    ok_ty Δ T.
   Proof.
     induction 1 as [ | | | | t σ def hσ hi hdef hconstr
-    | | | s t hs hi ht hit | s t hs hi ht hit | | | | ] => Γ Γ' heq hΓ; subst; try by constructor.
+    | | | s t hs hi ht hit | s t hs hi ht hit | | | | ] => Δ Δ' heq hΔ; subst; try by constructor.
     - apply OkClass with def => //.
       + move => i ty h; by eapply hi.
       + move => i c h.
-        apply subtype_constraint_elim with Γ'; by eauto.
+        apply subtype_constraint_elim with Δ'; by eauto.
     - constructor; by eauto.
     - constructor; by eauto.
   Qed.
 
-  Lemma ok_ty_constraint_elim Γ Γ' T:
-    ok_ty (Γ ++ Γ') T →
-    (∀ i c, Γ' !! i = Some c → Γ ⊢ c.1 <D: c.2) →
-    ok_ty Γ T.
+  Lemma ok_ty_constraint_elim Δ Δ' T:
+    ok_ty (Δ ++ Δ') T →
+    (∀ i c, Δ' !! i = Some c → Δ ⊢ c.1 <D: c.2) →
+    ok_ty Δ T.
   Proof. intros; by eapply ok_ty_constraint_elim_. Qed.
 
-  Lemma ok_ty_weaken Γ t: ok_ty Γ t → ∀ Γ', Γ ⊆ Γ' → ok_ty Γ' t.
+  Lemma ok_ty_weaken Δ t: ok_ty Δ t → ∀ Δ', Δ ⊆ Δ' → ok_ty Δ' t.
   Proof.
     induction 1 as [ | | | | t σ def hσ hi hdef hconstr
-    | | | s t hs hi ht hit | s t hs hi ht hit | n | t | | ] => Γ' hincl; try by constructor.
+    | | | s t hs hi ht hit | s t hs hi ht hit | n | t | | ] => Δ' hincl; try by constructor.
     - apply OkClass with def => //.
       + move => i ty h; by apply hi with i.
       + move => i c h.
-        apply subtype_weaken with Γ; by eauto.
+        apply subtype_weaken with Δ; by eauto.
     - constructor; by eauto.
     - constructor; by eauto.
   Qed.
 
-  Lemma ok_ty_class_inv Γ t σ: ok_ty Γ (ClassT t σ) → Forall (ok_ty Γ) σ.
+  Lemma ok_ty_class_inv Δ t σ: ok_ty Δ (ClassT t σ) → Forall (ok_ty Δ) σ.
   Proof.
     move => h; inv h.
     apply Forall_forall => x hin.
@@ -83,19 +83,19 @@ Section Typing.
     by eauto.
   Qed.
 
-  Lemma ok_ty_subst Γ t:
-    map_Forall (λ _, wf_cdef_parent Δ) Δ →
-    map_Forall (λ _, wf_cdef_constraints_bounded) Δ →
-    ok_ty Γ t →
+  Lemma ok_ty_subst Δ t:
+    map_Forall (λ _, wf_cdef_parent pdefs) pdefs →
+    map_Forall (λ _, wf_cdef_constraints_bounded) pdefs →
+    ok_ty Δ t →
     wf_ty t →
-    ∀ Γ' σ, Forall wf_ty σ →
-         Forall (ok_ty Γ') σ →
-         ok_ty (Γ' ++ (subst_constraints σ Γ)) (subst_ty σ t).
+    ∀ Δ' σ, Forall wf_ty σ →
+         Forall (ok_ty Δ') σ →
+         ok_ty (Δ' ++ (subst_constraints σ Δ)) (subst_ty σ t).
   Proof.
     move => hwp hcb.
     induction 1 as [ | | | | t σt def hσt hi hdef hconstr
     | | | s t hs his ht hit | s t hs his ht hit | n | t | | ]
-    => hwf Γ' σ hwfσ hokσ /=; try (constructor; by eauto).
+    => hwf Δ' σ hwfσ hokσ /=; try (constructor; by eauto).
     - apply OkClass with def => //.
       + move => i ty h.
         apply list_lookup_fmap_inv in h as [ty' [-> h]].
@@ -111,7 +111,7 @@ Section Typing.
         assert (h' := h).
         apply elem_of_list_lookup_2 in h.
         apply hdef' in h as [].
-        apply subtype_weaken with (subst_constraints σ Γ); last by set_solver.
+        apply subtype_weaken with (subst_constraints σ Δ); last by set_solver.
         rewrite -!subst_ty_subst.
         * apply subtype_subst => //.
           by apply hconstr with i.
@@ -127,14 +127,14 @@ Section Typing.
       simpl.
       rewrite Forall_forall in hokσ.
       apply elem_of_list_lookup_2 in hty.
-      apply ok_ty_weaken with Γ'; first by apply hokσ.
+      apply ok_ty_weaken with Δ'; first by apply hokσ.
       by set_solver.
   Qed.
 
-  Definition ok_constraint Γ (c: constraint) :=
-    ok_ty Γ c.1 ∧ ok_ty Γ c.2.
+  Definition ok_constraint Δ (c: constraint) :=
+    ok_ty Δ c.1 ∧ ok_ty Δ c.2.
 
-  Definition ok_constraints Γ G := Forall (ok_constraint Γ) G.
+  Definition ok_constraints Δ G := Forall (ok_constraint Δ) G.
 
   Definition wf_cdef_parent_ok cdef :=
     match cdef.(superclass) with
@@ -145,55 +145,55 @@ Section Typing.
   .
 
   Lemma extends_using_ok A B σ:
-    map_Forall (λ _cname, wf_cdef_parent_ok) Δ →
+    map_Forall (λ _cname, wf_cdef_parent_ok) pdefs →
     extends_using A B σ →
     ∃ adef,
-    Δ !! A = Some adef ∧
+    pdefs !! A = Some adef ∧
     ok_ty adef.(constraints) (ClassT B σ).
   Proof.
     move => hok h.
-    destruct h as [A B adef σ hΔ hsuper].
+    destruct h as [A B adef σ hpdefs hsuper].
     exists adef; split => //.
-    apply hok in hΔ.
-    by rewrite /wf_cdef_parent_ok hsuper in hΔ.
+    apply hok in hpdefs.
+    by rewrite /wf_cdef_parent_ok hsuper in hpdefs.
   Qed.
 
-  Lemma gen_targs_ok Γ n:
+  Lemma gen_targs_ok Δ n:
     ∀ i ty, gen_targs n !! i = Some ty →
-    ok_ty Γ ty.
+    ok_ty Δ ty.
   Proof.
     move => i ty /lookup_gen_targs ->.
     by constructor.
   Qed.
 
-  Lemma ok_ty_trans Γ ty:
-    ok_ty Γ ty →
-    ∀ Γ',
-    (∀ i c, Γ !! i = Some c → Γ' ⊢ c.1 <D: c.2) →
-    ok_ty Γ' ty.
+  Lemma ok_ty_trans Δ ty:
+    ok_ty Δ ty →
+    ∀ Δ',
+    (∀ i c, Δ !! i = Some c → Δ' ⊢ c.1 <D: c.2) →
+    ok_ty Δ' ty.
   Proof.
     induction 1 as [ | | | | t σ def hσ hi hdef hconstr
-    | | | s t hs hi ht hit | s t hs hi ht hit | n | t | | ] => Γ' hΓ; try by constructor.
+    | | | s t hs hi ht hit | s t hs hi ht hit | n | t | | ] => Δ' hΔ; try by constructor.
     - econstructor => //.
       + move => k ty hk; by eauto.
       + move => k c' hc'.
         apply hconstr in hc'.
-        apply subtype_constraint_trans with Γ; by eauto.
+        apply subtype_constraint_trans with Δ; by eauto.
     - constructor; by eauto.
     - constructor; by eauto.
   Qed.
 
   Lemma inherits_using_ok A B σ:
-    map_Forall (λ _ : string, wf_cdef_parent Δ) Δ →
-    map_Forall (λ _cname, wf_cdef_parent_ok) Δ →
-    map_Forall (λ _ : string, wf_cdef_constraints_bounded) Δ →
+    map_Forall (λ _ : string, wf_cdef_parent pdefs) pdefs →
+    map_Forall (λ _cname, wf_cdef_parent_ok) pdefs →
+    map_Forall (λ _ : string, wf_cdef_constraints_bounded) pdefs →
     inherits_using A B σ →
     ∃ adef,
-    Δ !! A = Some adef ∧
+    pdefs !! A = Some adef ∧
     ok_ty adef.(constraints) (ClassT B σ).
   Proof.
     move => hp hok hcb.
-    induction 1 as [ A adef hΔ | A B σ hext | A B σ C σC hext h hi ].
+    induction 1 as [ A adef hpdefs | A B σ hext | A B σ C σC hext h hi ].
     - exists adef; split => //.
       econstructor => //.
       + by apply gen_targs_ok.
@@ -202,14 +202,14 @@ Section Typing.
         * constructor.
           apply elem_of_list_lookup.
           exists i; by rewrite hc {1}(surjective_pairing c).
-        * apply hcb in hΔ.
-          rewrite /wf_cdef_constraints_bounded Forall_forall in hΔ.
+        * apply hcb in hpdefs.
+          rewrite /wf_cdef_constraints_bounded Forall_forall in hpdefs.
           apply elem_of_list_lookup_2 in hc.
-          by apply hΔ in hc as [].
-        * apply hcb in hΔ.
-          rewrite /wf_cdef_constraints_bounded Forall_forall in hΔ.
+          by apply hpdefs in hc as [].
+        * apply hcb in hpdefs.
+          rewrite /wf_cdef_constraints_bounded Forall_forall in hpdefs.
           apply elem_of_list_lookup_2 in hc.
-          by apply hΔ in hc as [].
+          by apply hpdefs in hc as [].
     - by apply extends_using_ok in hext.
     - destruct hi as (bdef & hB & hokB).
       assert (hwfB: wf_ty (ClassT B σ)).
@@ -221,7 +221,7 @@ Section Typing.
         by repeat destruct h as [? h].
       }
       inv hwfC.
-      destruct hext as [A B adef σ hΔ hsuper].
+      destruct hext as [A B adef σ hpdefs hsuper].
       exists adef; split => //.
       econstructor => //.
       { move => i ty hi.
@@ -231,9 +231,9 @@ Section Typing.
           { inv hokB; by eauto. }
           { by eauto. }
           { by apply wf_ty_class_inv in hwfB. }
-          apply hok in hΔ.
-          rewrite /wf_cdef_parent_ok hsuper in hΔ.
-          by apply ok_ty_class_inv in hΔ.
+          apply hok in hpdefs.
+          rewrite /wf_cdef_parent_ok hsuper in hpdefs.
+          by apply ok_ty_class_inv in hpdefs.
         + move => j c.
           rewrite lookup_app_Some.
           case => [hc | [? ]].
@@ -243,9 +243,9 @@ Section Typing.
           * rewrite /subst_constraints => hc.
             apply list_lookup_fmap_inv in hc as [c' [-> hc]].
             rewrite /subst_constraint /=.
-            apply hok in hΔ.
-            rewrite /wf_cdef_parent_ok hsuper in hΔ.
-            inv hΔ; simplify_eq.
+            apply hok in hpdefs.
+            rewrite /wf_cdef_parent_ok hsuper in hpdefs.
+            inv hpdefs; simplify_eq.
             by eauto.
       }
       move => i c hc.
@@ -257,9 +257,9 @@ Section Typing.
           rewrite /subst_constraints => hc'.
           apply list_lookup_fmap_inv in hc' as [c'' [-> hc']].
           rewrite /subst_constraint /=.
-          apply hok in hΔ.
-          rewrite /wf_cdef_parent_ok hsuper in hΔ.
-          inv hΔ; simplify_eq.
+          apply hok in hpdefs.
+          rewrite /wf_cdef_parent_ok hsuper in hpdefs.
+          inv hpdefs; simplify_eq.
           by eauto.
       + assert (hC := H1).
         apply hcb in hC.
@@ -282,8 +282,8 @@ Section Typing.
   Definition wf_cdef_constraints_ok cdef :=
     ok_constraints cdef.(constraints) cdef.(constraints).
 
-  Definition mdef_ok Γ mdef : Prop :=
-    map_Forall (λ _argname, ok_ty Γ) mdef.(methodargs) ∧ ok_ty Γ mdef.(methodrettype).
+  Definition mdef_ok Δ mdef : Prop :=
+    map_Forall (λ _argname, ok_ty Δ) mdef.(methodargs) ∧ ok_ty Δ mdef.(methodrettype).
 
   Definition cdef_methods_ok cdef :=
     map_Forall (λ _mname, mdef_ok cdef.(constraints)) cdef.(classmethods).
@@ -296,56 +296,56 @@ Section Typing.
     end
   .
 
-  Inductive expr_has_ty Γ (lty : local_tys):
+  Inductive expr_has_ty Δ (Γ : local_tys):
     subtype_kind → expr → lang_ty → Prop :=
-    | IntTy : ∀ kd z, expr_has_ty Γ lty kd (IntE z) IntT
-    | BoolTy: ∀ kd b, expr_has_ty Γ lty kd (BoolE b) BoolT
-    | NullTy kd: expr_has_ty Γ lty kd NullE NullT
+    | IntTy : ∀ kd z, expr_has_ty Δ Γ kd (IntE z) IntT
+    | BoolTy: ∀ kd b, expr_has_ty Δ Γ kd (BoolE b) BoolT
+    | NullTy kd: expr_has_ty Δ Γ kd NullE NullT
     | BinOpIntTy: ∀ kd op e1 e2,
         is_bool_op op = false →
-        expr_has_ty Γ lty kd e1 IntT →
-        expr_has_ty Γ lty kd e2 IntT →
-        expr_has_ty Γ lty kd (BinOpE op e1 e2) IntT
+        expr_has_ty Δ Γ kd e1 IntT →
+        expr_has_ty Δ Γ kd e2 IntT →
+        expr_has_ty Δ Γ kd (BinOpE op e1 e2) IntT
     | BinOpBoolTy: ∀ kd op e1 e2,
         is_bool_op op = true →
-        expr_has_ty Γ lty kd e1 IntT →
-        expr_has_ty Γ lty kd e2 IntT →
-        expr_has_ty Γ lty kd (BinOpE op e1 e2) BoolT
+        expr_has_ty Δ Γ kd e1 IntT →
+        expr_has_ty Δ Γ kd e2 IntT →
+        expr_has_ty Δ Γ kd (BinOpE op e1 e2) BoolT
     | EqBoolTy: ∀ kd e1 e2,
-        expr_has_ty Γ lty kd e1 BoolT →
-        expr_has_ty Γ lty kd e2 BoolT →
-        expr_has_ty Γ lty kd (BinOpE EqO e1 e2) BoolT
+        expr_has_ty Δ Γ kd e1 BoolT →
+        expr_has_ty Δ Γ kd e2 BoolT →
+        expr_has_ty Δ Γ kd (BinOpE EqO e1 e2) BoolT
     | UniOpTy: ∀ kd e,
-        expr_has_ty Γ lty kd e BoolT →
-        expr_has_ty Γ lty kd (UniOpE NotO e) BoolT
+        expr_has_ty Δ Γ kd e BoolT →
+        expr_has_ty Δ Γ kd (UniOpE NotO e) BoolT
     | GenTy: ∀ kd v ty,
-        lty.(ctxt) !! v = Some ty →
-        expr_has_ty Γ lty kd (VarE v) ty
-    | ThisTy kd: expr_has_ty Γ lty kd ThisE (this_type lty)
+        Γ.(ctxt) !! v = Some ty →
+        expr_has_ty Δ Γ kd (VarE v) ty
+    | ThisTy kd: expr_has_ty Δ Γ kd ThisE (this_type Γ)
     | ESubTy: ∀ kd e s t,
-        expr_has_ty Γ lty kd e s →
+        expr_has_ty Δ Γ kd e s →
         wf_ty t →
-        ok_ty Γ t →
-        subtype Γ kd s t →
-        expr_has_ty Γ lty kd e t
+        ok_ty Δ t →
+        subtype Δ kd s t →
+        expr_has_ty Δ Γ kd e t
     (* SD.V3 <D: is only available using explicit UpcastE *)
     | UpcastTy: ∀ kd e s t,
-        expr_has_ty Γ lty kd e s →
+        expr_has_ty Δ Γ kd e s →
         wf_ty t →
-        ok_ty Γ t →
-        Γ ⊢ s <D: t →
-        expr_has_ty Γ lty kd (UpcastE e t) t
+        ok_ty Δ t →
+        Δ ⊢ s <D: t →
+        expr_has_ty Δ Γ kd (UpcastE e t) t
   .
 
-  Lemma expr_has_ty_constraint_elim_ G kd lty e ty:
-    expr_has_ty G lty kd e ty →
-    ∀ Γ Γ', G = Γ ++ Γ' →
-    (∀ i c, Γ' !! i = Some c → Γ ⊢ c.1 <D: c.2) →
-    expr_has_ty Γ lty kd e ty.
+  Lemma expr_has_ty_constraint_elim_ G kd Γ e ty:
+    expr_has_ty G Γ kd e ty →
+    ∀ Δ Δ', G = Δ ++ Δ' →
+    (∀ i c, Δ' !! i = Some c → Δ ⊢ c.1 <D: c.2) →
+    expr_has_ty Δ Γ kd e ty.
   Proof.
     induction 1 as [ | | | kd op e1 e2 hop h1 hi1 h2 hi2 |
       kd op e1 e2 hop h1 hi1 h2 hi2 | kd e1 e2 h1 hi1 h2 hi2 | kd e h hi | kd v ty h | |
-      kd e s t h hi hok hsub | kd e s t h hi hok hsub] => Γ Γ' heq hΓ; subst; try (by constructor).
+      kd e s t h hi hok hsub | kd e s t h hi hok hsub] => Δ Δ' heq hΔ; subst; try (by constructor).
     - constructor; by eauto.
     - constructor; by eauto.
     - constructor; by eauto.
@@ -362,19 +362,19 @@ Section Typing.
       + by eapply subtype_constraint_elim.
   Qed.
 
-  Lemma expr_has_ty_constraint_elim Γ Γ' kd lty e ty:
-    expr_has_ty (Γ ++ Γ') lty kd e ty →
-    (∀ i c, Γ' !! i = Some c → Γ ⊢ c.1 <D: c.2) →
-    expr_has_ty Γ lty kd e ty.
+  Lemma expr_has_ty_constraint_elim Δ Δ' kd Γ e ty:
+    expr_has_ty (Δ ++ Δ') Γ kd e ty →
+    (∀ i c, Δ' !! i = Some c → Δ ⊢ c.1 <D: c.2) →
+    expr_has_ty Δ Γ kd e ty.
   Proof. intros; by eapply expr_has_ty_constraint_elim_. Qed.
 
-  Lemma expr_has_ty_subst Γ' Γ kd σ lty e ty:
-    map_Forall (λ _ : string, wf_cdef_parent Δ) Δ →
-    map_Forall (λ _ : string, wf_cdef_constraints_bounded) Δ →
+  Lemma expr_has_ty_subst Δ' Δ kd σ Γ e ty:
+    map_Forall (λ _ : string, wf_cdef_parent pdefs) pdefs →
+    map_Forall (λ _ : string, wf_cdef_constraints_bounded) pdefs →
     Forall wf_ty σ →
-    Forall (ok_ty Γ') σ →
-    expr_has_ty Γ lty kd e ty →
-    expr_has_ty (Γ' ++ (subst_constraints σ Γ)) (subst_lty σ lty) kd (subst_expr σ e) (subst_ty σ ty).
+    Forall (ok_ty Δ') σ →
+    expr_has_ty Δ Γ kd e ty →
+    expr_has_ty (Δ' ++ (subst_constraints σ Δ)) (subst_lty σ Γ) kd (subst_expr σ e) (subst_ty σ ty).
   Proof.
     move => hp hb hσwf hσok.
     induction 1 as [ | | | kd op e1 e2 hop h1 hi1 h2 hi2 |
@@ -386,24 +386,24 @@ Section Typing.
     - econstructor; first by apply hi.
       + by apply wf_ty_subst.
       + by apply ok_ty_subst.
-      + apply subtype_weaken with (subst_constraints σ Γ); first by apply subtype_subst.
+      + apply subtype_weaken with (subst_constraints σ Δ); first by apply subtype_subst.
         by set_solver.
     - eapply UpcastTy; first by apply hi.
       + by apply wf_ty_subst.
       + by apply ok_ty_subst.
-      + apply subtype_weaken with (subst_constraints σ Γ); first by apply subtype_subst.
+      + apply subtype_weaken with (subst_constraints σ Δ); first by apply subtype_subst.
         by set_solver.
   Qed.
 
-  Definition wf_lty lty :=
-    wf_ty (this_type lty) ∧
-    map_Forall (λ _, wf_ty) lty.(ctxt)
+  Definition wf_lty Γ :=
+    wf_ty (this_type Γ) ∧
+    map_Forall (λ _, wf_ty) Γ.(ctxt)
   .
 
-  Lemma insert_wf_lty x ty lty :
-    wf_ty ty → wf_lty lty → wf_lty (<[x := ty]>lty).
+  Lemma insert_wf_lty x ty Γ :
+    wf_ty ty → wf_lty Γ → wf_lty (<[x := ty]>Γ).
   Proof.
-    destruct lty as [[lt lσ] lty].
+    destruct Γ as [[lt lσ] Γ].
     rewrite /wf_lty /this_type /= => h [h0 hl]; split => //.
     rewrite map_Forall_lookup => k tk.
     rewrite lookup_insert_Some.
@@ -411,10 +411,10 @@ Section Typing.
     by apply hl in hk.
   Qed.
 
-  Lemma subst_wf_lty σ lty :
-    Forall wf_ty σ → wf_lty lty → wf_lty (subst_lty σ lty).
+  Lemma subst_wf_lty σ Γ :
+    Forall wf_ty σ → wf_lty Γ → wf_lty (subst_lty σ Γ).
   Proof.
-    destruct lty as [[lt lσ] lty].
+    destruct Γ as [[lt lσ] Γ].
     rewrite /wf_lty /this_type /= => hσ [h0 hl]; split.
     - inv h0.
       econstructor => //.
@@ -431,9 +431,9 @@ Section Typing.
       by apply hl in hk.
   Qed.
 
-  Lemma expr_has_ty_wf Γ kd lty e ty:
-    wf_lty lty →
-    expr_has_ty Γ lty kd e ty →
+  Lemma expr_has_ty_wf Δ kd Γ e ty:
+    wf_lty Γ →
+    expr_has_ty Δ Γ kd e ty →
     wf_ty ty.
   Proof.
     move => hwf.
@@ -445,7 +445,7 @@ Section Typing.
   Qed.
 
   (* continuation-based typing for commands.
-   * Γ is the set of constraints S <: T of the current class
+   * Δ is the set of constraints S <: T of the current class
    * and C is the tag of the current class (for `private` related checks)
    *
    * Note on Getter/Setter visibility check:
@@ -455,126 +455,126 @@ Section Typing.
    * is where the member is defined, and the member can only be accessed
    * via `This`
    *)
-  Inductive cmd_has_ty Γ (C : tag) : subtype_kind → local_tys → cmd → local_tys → Prop :=
-    | SkipTy: ∀ lty kd, cmd_has_ty Γ C kd lty SkipC lty
-    | ErrorTy: ∀ kd lty rty,
-        wf_lty rty → cmd_has_ty Γ C kd lty ErrorC rty
-    | SeqTy: ∀ kd lty1 lty2 lty3 fstc sndc,
-        cmd_has_ty Γ C kd lty1 fstc lty2 →
-        cmd_has_ty Γ C kd lty2 sndc lty3 →
-        cmd_has_ty Γ C kd lty1 (SeqC fstc sndc) lty3
-    | LetTy: ∀ kd lty lhs e ty,
-        expr_has_ty Γ lty kd e ty →
-        cmd_has_ty Γ C kd lty (LetC lhs e) (<[lhs := ty]>lty)
-    | IfTy: ∀ kd lty1 lty2 cond thn els,
-        expr_has_ty Γ lty1 kd cond BoolT →
-        cmd_has_ty Γ C kd lty1 thn lty2 →
-        cmd_has_ty Γ C kd lty1 els lty2 →
-        cmd_has_ty Γ C kd lty1 (IfC cond thn els) lty2
-    | GetPrivTy: ∀ kd lty lhs t σ name fty,
-        type_of_this lty = (t, σ) →
+  Inductive cmd_has_ty Δ (C : tag) : subtype_kind → local_tys → cmd → local_tys → Prop :=
+    | SkipTy: ∀ Γ kd, cmd_has_ty Δ C kd Γ SkipC Γ
+    | ErrorTy: ∀ kd Γ0 Γ1,
+        wf_lty Γ1 → cmd_has_ty Δ C kd Γ0 ErrorC Γ1
+    | SeqTy: ∀ kd Γ1 Γ2 Γ3 fstc sndc,
+        cmd_has_ty Δ C kd Γ1 fstc Γ2 →
+        cmd_has_ty Δ C kd Γ2 sndc Γ3 →
+        cmd_has_ty Δ C kd Γ1 (SeqC fstc sndc) Γ3
+    | LetTy: ∀ kd Γ lhs e ty,
+        expr_has_ty Δ Γ kd e ty →
+        cmd_has_ty Δ C kd Γ (LetC lhs e) (<[lhs := ty]>Γ)
+    | IfTy: ∀ kd Γ1 Γ2 cond thn els,
+        expr_has_ty Δ Γ1 kd cond BoolT →
+        cmd_has_ty Δ C kd Γ1 thn Γ2 →
+        cmd_has_ty Δ C kd Γ1 els Γ2 →
+        cmd_has_ty Δ C kd Γ1 (IfC cond thn els) Γ2
+    | GetPrivTy: ∀ kd Γ lhs t σ name fty,
+        type_of_this Γ = (t, σ) →
         has_field name t Private fty C →
-        cmd_has_ty Γ C kd lty (GetC lhs ThisE name) (<[lhs := subst_ty σ fty]>lty)
-    | GetPubTy: ∀ kd lty lhs recv t σ name fty orig,
-        expr_has_ty Γ lty kd recv (ClassT t σ) →
+        cmd_has_ty Δ C kd Γ (GetC lhs ThisE name) (<[lhs := subst_ty σ fty]>Γ)
+    | GetPubTy: ∀ kd Γ lhs recv t σ name fty orig,
+        expr_has_ty Δ Γ kd recv (ClassT t σ) →
         has_field name t Public fty orig →
-        cmd_has_ty Γ C kd lty (GetC lhs recv name) (<[lhs := subst_ty σ fty]>lty)
-    | SetPrivTy: ∀ kd lty fld rhs fty t σ,
-        type_of_this lty = (t, σ) →
+        cmd_has_ty Δ C kd Γ (GetC lhs recv name) (<[lhs := subst_ty σ fty]>Γ)
+    | SetPrivTy: ∀ kd Γ fld rhs fty t σ,
+        type_of_this Γ = (t, σ) →
         has_field fld t Private fty C →
-        expr_has_ty Γ lty kd rhs (subst_ty σ fty) →
-        cmd_has_ty Γ C kd lty (SetC ThisE fld rhs) lty
-    | SetPubTy: ∀ kd lty recv fld rhs fty orig t σ,
-        expr_has_ty Γ lty kd recv (ClassT t σ) →
+        expr_has_ty Δ Γ kd rhs (subst_ty σ fty) →
+        cmd_has_ty Δ C kd Γ (SetC ThisE fld rhs) Γ
+    | SetPubTy: ∀ kd Γ recv fld rhs fty orig t σ,
+        expr_has_ty Δ Γ kd recv (ClassT t σ) →
         has_field fld t Public fty orig →
-        expr_has_ty Γ lty kd rhs (subst_ty σ fty) →
-        cmd_has_ty Γ C kd lty (SetC recv fld rhs) lty
-    | NewTy: ∀ kd lty lhs t targs args fields,
+        expr_has_ty Δ Γ kd rhs (subst_ty σ fty) →
+        cmd_has_ty Δ C kd Γ (SetC recv fld rhs) Γ
+    | NewTy: ∀ kd Γ lhs t targs args fields,
         wf_ty (ClassT t targs) →
-        ok_ty Γ (ClassT t targs) →
+        ok_ty Δ (ClassT t targs) →
         has_fields t fields →
         dom fields = dom args →
         (∀ f fty arg,
         fields !! f = Some fty →
         args !! f = Some arg →
-        expr_has_ty Γ lty kd arg (subst_ty targs fty.1.2)) →
-        cmd_has_ty Γ C kd lty (NewC lhs t targs args) (<[lhs := ClassT t targs]>lty)
-    | CallTy: ∀ kd lty lhs recv t targs name orig mdef args,
-        expr_has_ty Γ lty kd recv (ClassT t targs) →
+        expr_has_ty Δ Γ kd arg (subst_ty targs fty.1.2)) →
+        cmd_has_ty Δ C kd Γ (NewC lhs t targs args) (<[lhs := ClassT t targs]>Γ)
+    | CallTy: ∀ kd Γ lhs recv t targs name orig mdef args,
+        expr_has_ty Δ Γ kd recv (ClassT t targs) →
         has_method name t orig mdef →
         dom mdef.(methodargs) = dom args →
         (∀ x ty arg,
         mdef.(methodargs) !! x = Some ty →
         args !! x = Some arg →
-        expr_has_ty Γ lty kd arg (subst_ty targs ty)) →
-        cmd_has_ty Γ C kd lty (CallC lhs recv name args) (<[lhs := subst_ty targs mdef.(methodrettype)]>lty)
-    | SubTy: ∀ kd lty c rty rty',
-        lty_sub Γ kd rty' rty →
-        cmd_has_ty Γ C kd lty c rty' →
-        cmd_has_ty Γ C kd lty c rty
-    | TagCheckTy kd lty rty v tv t thn els:
-        lty.(ctxt) !! v = Some tv →
-        cmd_has_ty Γ C kd (<[v:=InterT tv (ExT t)]> lty) thn rty →
-        cmd_has_ty Γ C kd lty els rty →
-        cmd_has_ty Γ C kd lty (RuntimeCheckC v (RCTag t) thn els) rty
-    | IntCheckTy kd lty rty v tv thn els:
-        lty.(ctxt) !! v = Some tv →
-        cmd_has_ty Γ C kd (<[v:=InterT tv IntT]> lty) thn rty →
-        cmd_has_ty Γ C kd lty els rty →
-        cmd_has_ty Γ C kd lty (RuntimeCheckC v RCInt thn els) rty
-    | BoolCheckTy kd lty rty v tv thn els:
-        lty.(ctxt) !! v = Some tv →
-        cmd_has_ty Γ C kd (<[v:=InterT tv BoolT]> lty) thn rty →
-        cmd_has_ty Γ C kd lty els rty →
-        cmd_has_ty Γ C kd lty (RuntimeCheckC v RCBool thn els) rty
-    | NullCheckTy kd lty rty v tv thn els:
-        lty.(ctxt) !! v = Some tv →
-        cmd_has_ty Γ C kd (<[v:=InterT tv NullT]> lty) thn rty →
-        cmd_has_ty Γ C kd lty els rty →
-        cmd_has_ty Γ C kd lty (RuntimeCheckC v RCNull thn els) rty
-    | NonNullCheckTy kd lty rty v tv thn els:
-        lty.(ctxt) !! v = Some tv →
-        cmd_has_ty Γ C kd (<[v:=InterT tv NonNullT]> lty) thn rty →
-        cmd_has_ty Γ C kd lty els rty →
-        cmd_has_ty Γ C kd lty (RuntimeCheckC v RCNonNull thn els) rty
+        expr_has_ty Δ Γ kd arg (subst_ty targs ty)) →
+        cmd_has_ty Δ C kd Γ (CallC lhs recv name args) (<[lhs := subst_ty targs mdef.(methodrettype)]>Γ)
+    | SubTy: ∀ kd Γ c Γ0 Γ1,
+        lty_sub Δ kd Γ1 Γ0 →
+        cmd_has_ty Δ C kd Γ c Γ1 →
+        cmd_has_ty Δ C kd Γ c Γ0
+    | TagCheckTy kd Γ0 Γ1 v tv t thn els:
+        Γ0.(ctxt) !! v = Some tv →
+        cmd_has_ty Δ C kd (<[v:=InterT tv (ExT t)]> Γ0) thn Γ1 →
+        cmd_has_ty Δ C kd Γ0 els Γ1 →
+        cmd_has_ty Δ C kd Γ0 (RuntimeCheckC v (RCTag t) thn els) Γ1
+    | IntCheckTy kd Γ0 Γ1 v tv thn els:
+        Γ0.(ctxt) !! v = Some tv →
+        cmd_has_ty Δ C kd (<[v:=InterT tv IntT]> Γ0) thn Γ1 →
+        cmd_has_ty Δ C kd Γ0 els Γ1 →
+        cmd_has_ty Δ C kd Γ0 (RuntimeCheckC v RCInt thn els) Γ1
+    | BoolCheckTy kd Γ0 Γ1 v tv thn els:
+        Γ0.(ctxt) !! v = Some tv →
+        cmd_has_ty Δ C kd (<[v:=InterT tv BoolT]> Γ0) thn Γ1 →
+        cmd_has_ty Δ C kd Γ0 els Γ1 →
+        cmd_has_ty Δ C kd Γ0 (RuntimeCheckC v RCBool thn els) Γ1
+    | NullCheckTy kd Γ0 Γ1 v tv thn els:
+        Γ0.(ctxt) !! v = Some tv →
+        cmd_has_ty Δ C kd (<[v:=InterT tv NullT]> Γ0) thn Γ1 →
+        cmd_has_ty Δ C kd Γ0 els Γ1 →
+        cmd_has_ty Δ C kd Γ0 (RuntimeCheckC v RCNull thn els) Γ1
+    | NonNullCheckTy kd Γ0 Γ1 v tv thn els:
+        Γ0.(ctxt) !! v = Some tv →
+        cmd_has_ty Δ C kd (<[v:=InterT tv NonNullT]> Γ0) thn Γ1 →
+        cmd_has_ty Δ C kd Γ0 els Γ1 →
+        cmd_has_ty Δ C kd Γ0 (RuntimeCheckC v RCNonNull thn els) Γ1
     (* Dynamic related typing rules *)
-    | DynIfTy: ∀ kd lty1 lty2 cond thn els,
-        expr_has_ty Γ lty1 kd cond DynamicT →
-        cmd_has_ty Γ C kd lty1 thn lty2 →
-        cmd_has_ty Γ C kd lty1 els lty2 →
-        cmd_has_ty Γ C kd lty1 (IfC cond thn els) lty2
-    | DynGetTy : ∀ kd lty lhs recv name,
-        expr_has_ty Γ lty kd recv DynamicT →
+    | DynIfTy: ∀ kd Γ1 Γ2 cond thn els,
+        expr_has_ty Δ Γ1 kd cond DynamicT →
+        cmd_has_ty Δ C kd Γ1 thn Γ2 →
+        cmd_has_ty Δ C kd Γ1 els Γ2 →
+        cmd_has_ty Δ C kd Γ1 (IfC cond thn els) Γ2
+    | DynGetTy : ∀ kd Γ lhs recv name,
+        expr_has_ty Δ Γ kd recv DynamicT →
         (match recv with
          | ThisE => False
          | _ => True
          end
         ) →
-        cmd_has_ty Γ C kd lty (GetC lhs recv name) (<[lhs := DynamicT]>lty)
-    | DynSetTy : ∀ kd lty recv fld rhs,
-        expr_has_ty Γ lty kd recv DynamicT →
-        expr_has_ty Γ lty kd rhs DynamicT →
+        cmd_has_ty Δ C kd Γ (GetC lhs recv name) (<[lhs := DynamicT]>Γ)
+    | DynSetTy : ∀ kd Γ recv fld rhs,
+        expr_has_ty Δ Γ kd recv DynamicT →
+        expr_has_ty Δ Γ kd rhs DynamicT →
         (match recv with
          | ThisE => False
          | _ => True
          end) →
-        cmd_has_ty Γ C kd lty (SetC recv fld rhs) lty
-    | DynCallTy: ∀ kd lty lhs recv name (args: stringmap expr),
-        expr_has_ty Γ lty kd recv DynamicT →
+        cmd_has_ty Δ C kd Γ (SetC recv fld rhs) Γ
+    | DynCallTy: ∀ kd Γ lhs recv name (args: stringmap expr),
+        expr_has_ty Δ Γ kd recv DynamicT →
         (∀ x arg, args !! x = Some arg →
-          expr_has_ty Γ lty kd arg DynamicT) →
+          expr_has_ty Δ Γ kd arg DynamicT) →
         (match recv with
          | ThisE => False
          | _ => True
          end) →
-        cmd_has_ty Γ C kd lty (CallC lhs recv name args) (<[lhs := DynamicT]>lty)
+        cmd_has_ty Δ C kd Γ (CallC lhs recv name args) (<[lhs := DynamicT]>Γ)
   .
 
-  Lemma cmd_has_ty_constraint_elim_ G C kd lty cmd rty:
-    cmd_has_ty G C kd lty cmd rty →
-    ∀ Γ Γ', G = Γ ++ Γ' →
-    (∀ i c, Γ' !! i = Some c → Γ ⊢ c.1 <D: c.2) →
-    cmd_has_ty Γ C kd lty cmd rty.
+  Lemma cmd_has_ty_constraint_elim_ G C kd Γ0 cmd Γ1:
+    cmd_has_ty G C kd Γ0 cmd Γ1 →
+    ∀ Δ Δ', G = Δ ++ Δ' →
+    (∀ i c, Δ' !! i = Some c → Δ ⊢ c.1 <D: c.2) →
+    cmd_has_ty Δ C kd Γ0 cmd Γ1.
   Proof.
     induction 1 as [ | ???? | ?????? h1 hi1 h2 hi2 | ????? he |
       ?????? he h1 hi1 h2 hi2 | ??????? he hf | ????????? he hf |
@@ -585,7 +585,7 @@ Section Typing.
       ??????? hin hthn hi0 hels hi1 | ??????? hin hthn hi0 helse hi1 |
       ?????? hcond hthn hi1 hels hi2 | ????? he hnotthis |
       ????? hrecv hrhs hnotthis | ?????? he hargs hnotthis
-      ] => Γ Γ' heq hΓ; subst.
+      ] => Δ Δ' heq hΔ; subst.
     - by econstructor.
     - by eapply ErrorTy.
     - econstructor; by eauto.
@@ -634,22 +634,22 @@ Section Typing.
         by eapply hargs.
   Qed.
 
-  Lemma cmd_has_ty_constraint_elim Γ Γ' C kd lty cmd rty:
-    cmd_has_ty (Γ ++ Γ') C kd lty cmd rty →
-    (∀ i c, Γ' !! i = Some c → Γ ⊢ c.1 <D: c.2) →
-    cmd_has_ty Γ C kd lty cmd rty.
+  Lemma cmd_has_ty_constraint_elim Δ Δ' C kd Γ0 cmd Γ1:
+    cmd_has_ty (Δ ++ Δ') C kd Γ0 cmd Γ1 →
+    (∀ i c, Δ' !! i = Some c → Δ ⊢ c.1 <D: c.2) →
+    cmd_has_ty Δ C kd Γ0 cmd Γ1.
   Proof. intros; by eapply cmd_has_ty_constraint_elim_. Qed.
 
-  Lemma cmd_has_ty_wf Γ C kd lty cmd lty' :
-    map_Forall (λ _ : string, wf_cdef_parent Δ) Δ →
-    map_Forall (λ _ : string, wf_cdef_fields_wf) Δ →
-    map_Forall (λ _ : string, wf_cdef_methods_wf) Δ →
-    Forall wf_constraint Γ →
-    wf_lty lty →
-    cmd_has_ty Γ C kd lty cmd lty' →
-    wf_lty lty'.
+  Lemma cmd_has_ty_wf Δ C kd Γ0 cmd Γ1:
+    map_Forall (λ _ : string, wf_cdef_parent pdefs) pdefs →
+    map_Forall (λ _ : string, wf_cdef_fields_wf) pdefs →
+    map_Forall (λ _ : string, wf_cdef_methods_wf) pdefs →
+    Forall wf_constraint Δ →
+    wf_lty Γ0 →
+    cmd_has_ty Δ C kd Γ0 cmd Γ1 →
+    wf_lty Γ1.
   Proof.
-    move => hp hfields hmethods hΓ [hthis hwf].
+    move => hp hfields hmethods hΔ [hthis hwf].
     induction 1 as [ | ???? | ?????? h1 hi1 h2 hi2 | ????? he |
       ?????? he h1 hi1 h2 hi2 | ??????? he hf | ????????? he hf |
       ??????? he hf hr | ????????? he hf hr | ??????? ht hok hf hdom hargs |
@@ -667,7 +667,7 @@ Section Typing.
       by apply expr_has_ty_wf in he.
     - apply insert_wf_lty => //.
       apply wf_ty_subst; last by apply has_field_wf in hf.
-      destruct lty as [[? ?] lty].
+      destruct Γ as [[? ?] Γ].
       rewrite /this_type /= in hthis, he.
       simplify_eq.
       by apply wf_ty_class_inv in hthis.
@@ -696,21 +696,21 @@ Section Typing.
     - by apply insert_wf_lty.
   Qed.
 
-  Lemma cmd_has_ty_subst Γ' Γ C kd σ lty cmd lty':
-    map_Forall (λ _ : string, wf_cdef_parent Δ) Δ →
-    map_Forall (λ _ : string, wf_cdef_fields_wf) Δ →
-    map_Forall (λ _ : string, wf_cdef_methods_wf) Δ →
-    map_Forall (λ _ : string, wf_cdef_fields_bounded) Δ →
-    map_Forall (λ _ : string, cdef_methods_bounded) Δ →
-    map_Forall (λ _ : string, wf_cdef_constraints_bounded) Δ →
-    Forall wf_constraint Γ →
-    wf_lty lty →
+  Lemma cmd_has_ty_subst Δ' Δ C kd σ Γ0 cmd Γ1:
+    map_Forall (λ _ : string, wf_cdef_parent pdefs) pdefs →
+    map_Forall (λ _ : string, wf_cdef_fields_wf) pdefs →
+    map_Forall (λ _ : string, wf_cdef_methods_wf) pdefs →
+    map_Forall (λ _ : string, wf_cdef_fields_bounded) pdefs →
+    map_Forall (λ _ : string, cdef_methods_bounded) pdefs →
+    map_Forall (λ _ : string, wf_cdef_constraints_bounded) pdefs →
+    Forall wf_constraint Δ →
+    wf_lty Γ0 →
     Forall wf_ty σ →
-    Forall (ok_ty Γ') σ →
-    cmd_has_ty Γ C kd lty cmd lty' →
-    cmd_has_ty (Γ' ++ (subst_constraints σ Γ)) C kd (subst_lty σ lty) (subst_cmd σ cmd) (subst_lty σ lty').
+    Forall (ok_ty Δ') σ →
+    cmd_has_ty Δ C kd Γ0 cmd Γ1 →
+    cmd_has_ty (Δ' ++ (subst_constraints σ Δ)) C kd (subst_lty σ Γ0) (subst_cmd σ cmd) (subst_lty σ Γ1).
   Proof.
-    move => hp hfields hmethods hfb hmb hcb hΓ hwf0 hwf1 hwf2.
+    move => hp hfields hmethods hfb hmb hcb hΔ hwf0 hwf1 hwf2.
     induction 1 as [ | ???? | ?????? h1 hi1 h2 hi2 | ????? he |
       ?????? he h1 hi1 h2 hi2 | ??????? he hf | ????????? he hf |
       ??????? he hf hr | ????????? he hf hr | ??????? hwf hok hf hdom hargs |
@@ -736,7 +736,7 @@ Section Typing.
         by eapply expr_has_ty_subst.
       + by apply hi1.
       + by apply hi2.
-    - destruct lty as [[this σt] lty].
+    - destruct Γ as [[this σt] Γ].
       destruct hwf0 as [hthis hwf].
       simpl in *.
       rewrite /this_type /= in hthis, he.
@@ -763,7 +763,7 @@ Section Typing.
       + rewrite -subst_ty_subst; first by eapply expr_has_ty_subst.
         apply has_field_bounded in hf => //.
         destruct hf as (hdef & ht & hfty).
-        destruct lty as [this lty]; simpl in he.
+        destruct Γ as [this Γ]; simpl in he.
         rewrite he in hwf0; destruct hwf0 as [hwf _].
         rewrite /this_type /= in hwf.
         inv hwf; simplify_eq.
@@ -847,13 +847,13 @@ Section Typing.
         inv he; simplify_eq.
         by rewrite H4.
     - econstructor; last by apply hi.
-      apply lty_sub_weaken with (subst_constraints σ Γ); last by set_solver.
+      apply lty_sub_weaken with (subst_constraints σ Δ); last by set_solver.
       by apply lty_sub_subst.
     - eapply TagCheckTy.
       + by rewrite lookup_fmap hin /=.
       + rewrite /subst_lty fmap_insert /= in hi0.
         apply hi0 => //.
-        destruct lty as [[lt lσ] lty].
+        destruct Γ0 as [[lt lσ] Γ0].
         split.
         * rewrite /this_type /=.
           by apply hwf0.
@@ -865,7 +865,7 @@ Section Typing.
       + by rewrite lookup_fmap hin /=.
       + rewrite /subst_lty fmap_insert /= in hi0.
         apply hi0 => //.
-        destruct lty as [[lt lσ] lty].
+        destruct Γ0 as [[lt lσ] Γ0].
         split.
         * rewrite /this_type /=.
           by apply hwf0.
@@ -877,7 +877,7 @@ Section Typing.
       + by rewrite lookup_fmap hin /=.
       + rewrite /subst_lty fmap_insert /= in hi0.
         apply hi0 => //.
-        destruct lty as [[lt lσ] lty].
+        destruct Γ0 as [[lt lσ] Γ0].
         split.
         * rewrite /this_type /=.
           by apply hwf0.
@@ -889,7 +889,7 @@ Section Typing.
       + by rewrite lookup_fmap hin /=.
       + rewrite /subst_lty fmap_insert /= in hi0.
         apply hi0 => //.
-        destruct lty as [[lt lσ] lty].
+        destruct Γ0 as [[lt lσ] Γ0].
         split.
         * rewrite /this_type /=.
           by apply hwf0.
@@ -901,7 +901,7 @@ Section Typing.
       + by rewrite lookup_fmap hin /=.
       + rewrite /subst_lty fmap_insert /= in hi0.
         apply hi0 => //.
-        destruct lty as [[lt lσ] lty].
+        destruct Γ0 as [[lt lσ] Γ0].
         split.
         * rewrite /this_type /=.
           by apply hwf0.
@@ -914,8 +914,8 @@ Section Typing.
         by eapply expr_has_ty_subst.
       + by apply hi1.
       + by apply hi2.
-    - replace (subst_lty σ (<[lhs:=DynamicT]> lty)) with
-             (<[lhs := DynamicT]>(subst_lty σ lty)); last first.
+    - replace (subst_lty σ (<[lhs:=DynamicT]> Γ)) with
+             (<[lhs := DynamicT]>(subst_lty σ Γ)); last first.
       { rewrite /subst_lty /= /insert /local_tys_insert /=.
         f_equal.
         by rewrite fmap_insert.
@@ -930,8 +930,8 @@ Section Typing.
       + change DynamicT with (subst_ty σ DynamicT).
         by eapply expr_has_ty_subst.
       + by destruct recv.
-    - replace (subst_lty σ (<[lhs:=DynamicT]> lty)) with
-             (<[lhs := DynamicT]>(subst_lty σ lty)); last first.
+    - replace (subst_lty σ (<[lhs:=DynamicT]> Γ)) with
+             (<[lhs := DynamicT]>(subst_lty σ Γ)); last first.
       { rewrite /subst_lty /= /insert /local_tys_insert /=.
         f_equal.
         by rewrite fmap_insert.
@@ -952,13 +952,13 @@ Section Typing.
    * method bodies must be well-formed under a generic substitution mapping
    * Ti -> Ti.
    *)
-  Definition wf_mdef_ty Γ tag σ mdef :=
-    ∃ rty,
-    wf_lty rty ∧
-    cmd_has_ty Γ tag Plain
+  Definition wf_mdef_ty Δ tag σ mdef :=
+    ∃ Γ',
+    wf_lty Γ' ∧
+    cmd_has_ty Δ tag Plain
       {| type_of_this := (tag, σ); ctxt := subst_ty σ <$> mdef.(methodargs) |}
-      mdef.(methodbody) rty ∧
-    expr_has_ty Γ rty Plain mdef.(methodret) (subst_ty σ mdef.(methodrettype))
+      mdef.(methodbody) Γ' ∧
+    expr_has_ty Δ Γ' Plain mdef.(methodret) (subst_ty σ mdef.(methodrettype))
   .
 
   Definition cdef_wf_mdef_ty cname cdef :=
@@ -969,13 +969,13 @@ Section Typing.
   (* Checks related to support dynamic *)
   Definition to_dyn (ty: lang_ty) : lang_ty := DynamicT.
 
-  Definition wf_mdef_dyn_ty Γ tag σ mdef :=
-    ∃ rty,
-    wf_lty rty ∧
-    cmd_has_ty Γ tag Aware
+  Definition wf_mdef_dyn_ty Δ tag σ mdef :=
+    ∃ Γ',
+    wf_lty Γ' ∧
+    cmd_has_ty Δ tag Aware
       {| type_of_this := (tag, σ); ctxt := to_dyn <$> mdef.(methodargs) |}
-      mdef.(methodbody) rty ∧
-    expr_has_ty Γ rty Aware mdef.(methodret) (to_dyn mdef.(methodrettype))
+      mdef.(methodbody) Γ' ∧
+    expr_has_ty Δ Γ' Aware mdef.(methodret) (to_dyn mdef.(methodrettype))
   .
 
   Definition wf_cdef_methods_dyn_wf cname cdef :=
@@ -993,11 +993,11 @@ Section Typing.
       else True) cdef.(classmethods)
   .
 
-  Definition wf_field_dyn_wf Σc (vfty: ((visibility * lang_ty) * tag)) :=
+  Definition wf_field_dyn_wf Δ (vfty: ((visibility * lang_ty) * tag)) :=
     match vfty.1 with
     | (Private, _) => True
     | (Public, fty) =>
-        Σc ⊢ fty <D: DynamicT ∧ Σc ⊢ DynamicT <D: fty
+        Δ ⊢ fty <D: DynamicT ∧ Δ ⊢ DynamicT <D: fty
     end.
 
   Definition wf_cdef_fields_dyn_wf cname cdef :=
@@ -1009,19 +1009,19 @@ Section Typing.
   Definition wf_cdef_dyn_parent cdef :=
     match cdef.(superclass) with
     | Some (parent, _) =>
-        ∀ def, Δ !! parent = Some def →
+        ∀ def, pdefs !! parent = Some def →
         def.(support_dynamic) = true →
         cdef.(support_dynamic) = true
     | None => True
     end.
 
   Lemma extends_using_dyn_parent A B σ:
-    map_Forall (λ _, wf_cdef_parent Δ) Δ →
-    map_Forall (λ _, wf_cdef_dyn_parent) Δ →
+    map_Forall (λ _, wf_cdef_parent pdefs) pdefs →
+    map_Forall (λ _, wf_cdef_dyn_parent) pdefs →
     extends_using A B σ →
     ∃ adef bdef,
-      Δ !! A = Some adef ∧
-      Δ !! B = Some bdef ∧
+      pdefs !! A = Some adef ∧
+      pdefs !! B = Some bdef ∧
       (bdef.(support_dynamic) = true → adef.(support_dynamic) = true).
   Proof.
     move => hp hwf hext.
@@ -1037,16 +1037,16 @@ Section Typing.
   Qed.
 
   Lemma inherits_using_dyn_parent A B σ:
-    map_Forall (λ _, wf_cdef_parent Δ) Δ →
-    map_Forall (λ _, wf_cdef_dyn_parent) Δ →
+    map_Forall (λ _, wf_cdef_parent pdefs) pdefs →
+    map_Forall (λ _, wf_cdef_dyn_parent) pdefs →
     inherits_using A B σ →
     ∃ adef bdef,
-      Δ !! A = Some adef ∧
-      Δ !! B = Some bdef ∧
+      pdefs !! A = Some adef ∧
+      pdefs !! B = Some bdef ∧
       (bdef.(support_dynamic) = true → adef.(support_dynamic) = true).
   Proof.
     move => hp hwf.
-    induction 1 as [ A adef hΔ | A B σ hext | A B σ C σC hext h hi ].
+    induction 1 as [ A adef hpdefs | A B σ hext | A B σ C σC hext h hi ].
     - exists adef, adef.
       by repeat split => //.
     - by apply extends_using_dyn_parent in hext.
@@ -1102,41 +1102,41 @@ Section MethodTyping.
   (* assume a given set of class definitions *)
   Context `{PDC: ProgDefContext}.
 
-  (* Helping the inference with this notation that hides Δ *)
-  Local Notation "Γ ⊢ s <: t" := (@subtype _ Γ Plain s t) (at level 70, s at next level, no associativity).
-  Local Notation "Γ ⊢ s <D: t" := (@subtype _ Γ Aware s t) (at level 70, s at next level, no associativity).
+  (* Helping the inference with this notation that hides pdefs *)
+  Local Notation "Δ ⊢ s <: t" := (@subtype _ Δ Plain s t) (at level 70, s at next level, no associativity).
+  Local Notation "Δ ⊢ s <D: t" := (@subtype _ Δ Aware s t) (at level 70, s at next level, no associativity).
 
   (* Let's consider that class C0 has/inherits a method m from class C1
    * where it is declared. Then m is correctly typed in C0 for any valid
    * instantiation of the class.
    *)
-  Lemma wf_mdef_ty_gen Σc C m σ def mdef:
-    wf_cdefs Δ →
-    Δ !! C = Some def →
+  Lemma wf_mdef_ty_gen Δ C m σ def mdef:
+    wf_cdefs pdefs →
+    pdefs !! C = Some def →
     def.(classmethods) !! m = Some mdef →
-    wf_ty (ClassT C σ) → ok_ty Σc (ClassT C σ) →
-    ∃ rty, wf_lty rty ∧
-      cmd_has_ty Σc C Plain {| type_of_this := (C, σ); ctxt := subst_ty σ <$> mdef.(methodargs) |}
-                (subst_cmd σ mdef.(methodbody)) rty ∧
-      expr_has_ty Σc rty Plain (subst_expr σ mdef.(methodret)) (subst_ty σ mdef.(methodrettype)).
+    wf_ty (ClassT C σ) → ok_ty Δ (ClassT C σ) →
+    ∃ Γ', wf_lty Γ' ∧
+      cmd_has_ty Δ C Plain {| type_of_this := (C, σ); ctxt := subst_ty σ <$> mdef.(methodargs) |}
+                (subst_cmd σ mdef.(methodbody)) Γ' ∧
+      expr_has_ty Δ Γ' Plain (subst_expr σ mdef.(methodret)) (subst_ty σ mdef.(methodrettype)).
   Proof.
-    move => hΔ hdef hmdef hwf hok.
-    destruct hΔ.
+    move => hpdefs hdef hmdef hwf hok.
+    destruct hpdefs.
     (* Let's assert a bunch of helper statements *)
     assert (hwfσ : Forall wf_ty σ) by (by apply wf_ty_class_inv in hwf).
-    assert (hokσ : Forall (ok_ty Σc) σ) by (by apply ok_ty_class_inv in hok).
+    assert (hokσ : Forall (ok_ty Δ) σ) by (by apply ok_ty_class_inv in hok).
     (* Let's use the general substitution lemma to make the instantiation *)
-    assert (hgen : ∃ rty, wf_lty rty ∧
-      cmd_has_ty (Σc ++ subst_constraints σ def.(constraints)) C Plain
+    assert (hgen : ∃ Γ', wf_lty Γ' ∧
+      cmd_has_ty (Δ ++ subst_constraints σ def.(constraints)) C Plain
                  (subst_lty σ {| type_of_this := (C, gen_targs (length def.(generics))); ctxt := mdef.(methodargs) |})
-                 (subst_cmd σ mdef.(methodbody)) rty ∧
-      expr_has_ty (Σc ++ subst_constraints σ def.(constraints))
-                  rty Plain (subst_expr σ mdef.(methodret)) (subst_ty σ mdef.(methodrettype))).
+                 (subst_cmd σ mdef.(methodbody)) Γ' ∧
+      expr_has_ty (Δ ++ subst_constraints σ def.(constraints))
+                  Γ' Plain (subst_expr σ mdef.(methodret)) (subst_ty σ mdef.(methodrettype))).
     { assert (hd := hdef).
       assert (hm := hmdef).
       apply wf_mdefs0 in hd.
-      apply hd in hm as [rty [wf_rty [hbody hret]]].
-      exists (subst_lty σ rty); split; last split.
+      apply hd in hm as [Γ' [wf_Γ' [hbody hret]]].
+      exists (subst_lty σ Γ'); split; last split.
       - by apply subst_wf_lty.
       - apply cmd_has_ty_subst => //.
         { assert (hd1 := hdef).
@@ -1164,20 +1164,20 @@ Section MethodTyping.
         apply hdef in hmdef.
         by apply hmdef.
     }
-    destruct hgen as (rty & hwf_rty & hbody & hret).
+    destruct hgen as (Γ' & hwf_Γ' & hbody & hret).
     (* Now, because everything is correctly typed, let's discharge
      * some redundant constraints.
      *)
     assert (hconstraints: ∀ i c,
       (subst_constraints σ (constraints def)) !! i = Some c →
-      Σc ⊢ c.1 <D: c.2).
+      Δ ⊢ c.1 <D: c.2).
     { move => i c hin.
       apply list_lookup_fmap_inv in hin as [c' [-> hin]].
       inv hok; simplify_eq.
       rewrite /subst_constraint /=.
       by eauto.
     }
-    exists rty; split; first done.
+    exists Γ'; split; first done.
     split.
     - eapply cmd_has_ty_constraint_elim => //.
       rewrite /subst_lty subst_ty_gen_targs //= in hbody.
